docs/README.md
@@ -4,4 +4,3 @@ Docs index;
 2. [Usage Instructions](USAGE.md)
 3. [Usage example](UsageExample.md)
 4. [Software Design Document](SWDD.md)
-5. [Publishing](PUBLISHING.md)
